src/spred.v
@@ -3,5 +3,6 @@
 Require Export x86proved.spred.core.
 Require Export x86proved.spred.stateis.
 Require Export x86proved.spred.tactics.
+Require Export x86proved.spred.memis.
 (* Important: the ssimpl tactic in pointsto overrides the one in septac *)
 Require Export x86proved.spred.pointsto.
