src/spred/memis.v
@@ -1,0 +1,648 @@
+(*===========================================================================
+    Mem-is predicates
+  ===========================================================================*)
+Require Import Ssreflect.ssreflect Ssreflect.ssrbool Ssreflect.ssrnat Ssreflect.ssrfun Ssreflect.eqtype Ssreflect.tuple Ssreflect.seq Ssreflect.choice Ssreflect.fintype.
+Require Import x86proved.bitsrep x86proved.bitsops x86proved.bitsprops x86proved.bitsopsprops x86proved.x86.procstate x86proved.x86.addr.
+Require Import x86proved.monad x86proved.reader x86proved.writer x86proved.roundtrip x86proved.spred.core x86proved.spred.stateis x86proved.spred.tactics x86proved.pfun x86proved.cursor x86proved.charge.iltac x86proved.charge.ilogic.
+
+Set Implicit Arguments.
+Unset Strict Implicit.
+Import Prenex Implicits.
+
+(*---------------------------------------------------------------------------
+   The intended meaning of
+      p -- q :-> v
+   is that the memory from p inclusive to q exclusive represents the value v.
+
+   We require that memIs p q v implies p<=q.
+  ---------------------------------------------------------------------------*)
+Class MemIs T := {
+  memIs:> ADDRCursor -> ADDRCursor -> T -> SPred;
+  memIsLe :> forall p q v, memIs p q v |-- leCursor p q /\\ memIs p q v
+}.
+
+Notation "p '--' q ':->' x" := (memIs p q x) (at level 50, q at next level, no associativity).
+
+(* This is a consequence of memIsLe *)
+Lemma memIsNonTop T {_:MemIs T} (v: T) (p: ADDRCursor) (q:ADDR) :
+    p -- q :-> v |-- Exists p':ADDR, p = mkCursor p' /\\ p -- q :-> v.
+Proof. eapply lentailsPre. apply memIsLe.
+sdestruct => H. elim (leCursorNonTop H) => [p' EQ].
+apply lexistsR with p'. rewrite EQ. sbazooka.
+Qed.
+
+(* This is another consequence of memIsLe *)
+(* We leave the argument to [top] unspecified so that it may be picked up as a constant an not be a numeral. *)
+Lemma memIsFromTop T (_:MemIs T) (v: T) (q: ADDR) :
+  top _ -- q :-> v |-- lfalse.
+Proof. rewrite -> memIsLe. rewrite /leCursor. by apply lpropandL. Qed.
+
+(* Our characterisation of fixed-size encodings *)
+Class FixedMemIs T n `(MI: MemIs T) :=
+  memIsFixed:> forall p q v, p -- q :-> v |-- apart n p q /\\ p -- q :-> v.
+
+(*---------------------------------------------------------------------------
+   We can interpret reader terms purely logically, using the primitive
+   byteIs predicate and separating conjunction.
+  ---------------------------------------------------------------------------*)
+Fixpoint interpReader T (rt:Reader T) (p q: ADDRCursor) (v: T) :=
+  match rt with
+  | readerRetn x =>
+    v = x /\\ p = q /\\ empSP
+
+  | readerNext rd =>
+    (* We can't read beyond the last byte of memory! *)
+    if p is mkCursor p'
+    then Exists b, byteIs p' b ** interpReader (rd b) (next p') q v
+    else lfalse
+
+  | readerSkip rd =>
+    if p is mkCursor p'
+    then Exists b, byteIs p' b ** interpReader rd (next p') q v
+    else lfalse
+
+  | readerCursor rd =>
+    interpReader (rd p) p q v
+  end.
+
+Lemma interpReader_entails_leCursor T (rt: Reader T) :
+  forall p q v, interpReader rt p q v |-- leCursor p q /\\ interpReader rt p q v.
+Proof. elim rt; rewrite /interpReader-/interpReader.
+- move => v p q w. sdestructs => -> ->. rewrite leCursor_refl. sbazooka.
+- move => rd IH p q w. elim p => //. move => d. sdestructs => byte.
+  rewrite -> IH. rewrite leCursor_next. sdestructs => LT. rewrite (leCursor_weaken LT).
+  sbazooka.
+- move => rd IH p q w. elim p => //. move => d. sdestructs => byte.
+  rewrite -> IH. rewrite leCursor_next. sdestructs => LT. rewrite (leCursor_weaken LT).
+  sbazooka.
+- move => rd IH p q v. apply IH.
+Qed.
+
+Lemma interpReader_retn T (v w:T) p q:
+  interpReader (retn v) p q w -|- p = q /\\ v = w /\\ empSP.
+Proof. simpl (retn _). rewrite /interpReader-/interpReader.
+sbazooka.
+Qed.
+
+Lemma interpReader_bind T1 T2 (r1: Reader T1) : forall (r2: T1 -> Reader T2) w p q,
+  interpReader (readerBind r1 r2) p q w -|-
+  Exists p', Exists v, interpReader r1 p p' v ** interpReader (r2 v) p' q w.
+Proof. induction r1 => r2 w p q.
++ rewrite /readerBind/interpReader-/interpReader. split.
+  * sbazooka.
+  * sdestructs => ? ? -> ->. sbazooka.
++ simpl readerBind. rewrite /interpReader-/interpReader.
+  destruct p.
+  * split.
+      sdestructs => byte. rewrite H. sbazooka.
+      sdestructs => p' v byte. setoid_rewrite H. sbazooka.
+  * sbazooka.
+(* readerSkip *)
++ simpl readerBind. rewrite /interpReader-/interpReader.
+  destruct p.
+  * split.
+      sdestructs => byte. rewrite IHr1. sbazooka.
+      sdestructs => p' v byte. setoid_rewrite IHr1. sbazooka.
+  * sbazooka.
+(* readerCursor *)
+  rewrite /readerBind-/readerBind/interpReader-/interpReader.
+  destruct p => //.
+Qed.
+
+Lemma interpReader_letPair T X Y (v:X*Y) (r: X -> Y -> Reader T) :
+  interpReader (let (x,y) := v in r x y) = interpReader (r v.1 v.2).
+Proof. by elim v. Qed.
+
+(*---------------------------------------------------------------------------
+  Typically we use interpReader to instantiate MemIs
+  ---------------------------------------------------------------------------*)
+Instance readerMemIs R {r:Reader R} : MemIs R :=
+  @Build_MemIs _ (interpReader readNext) (@interpReader_entails_leCursor R r).
+
+Lemma interpReaderPair T1 T2 (r1: Reader T1) (r2: Reader T2) v1 v2 p r :
+  Exists q, interpReader r1 p q v1 ** interpReader r2 q r v2 -|-
+  interpReader (let! x1 = r1; let! x2 = r2; retn (x1, x2)) p r (v1,v2).
+Proof. rewrite interpReader_bind.
+split.
++ sdestructs => q. sbazooka. sbazooka. rewrite interpReader_bind. sbazooka.
+  simpl. sbazooka.
++ sdestructs => p' v. rewrite interpReader_bind. sdestructs => p'' v'.
+  rewrite interpReader_retn. sdestructs => -> [-> ->]. sbazooka.
+Qed.
+
+Lemma readerMemIsSimpl R {r: Reader R} p q (v: R) :
+  p -- q :-> v -|- interpReader r p q v.
+Proof. by rewrite /memIs/=/readNext. Qed.
+
+Definition fixedSizeReader R (r: Reader R) n :=
+  forall p q v, interpReader r p q v |-- apart n p q /\\ interpReader r p q v.
+
+(*---------------------------------------------------------------------------
+   readerMemIs for bytes
+  ---------------------------------------------------------------------------*)
+
+Lemma interpReader_bindBYTE T (r: BYTE -> Reader T) w (p:ADDR) (q:ADDRCursor) :
+  interpReader (readerBind readNext r) p q w -|-
+  Exists b:BYTE, byteIs p b ** interpReader (r b) (next p) q w.
+Proof. rewrite interpReader_bind/readNext/readBYTE/interpReader-/interpReader.
+split. sbazooka. sbazooka. subst. by ssimpl. sbazooka.
+Qed.
+
+Lemma interpReader_bindBYTE_top T (r: BYTE -> Reader T) w (q:ADDRCursor) :
+  interpReader (readerBind readNext r) (top _) q w -|-
+  lfalse.
+Proof.
+rewrite interpReader_bind/readNext/readBYTE/interpReader-/interpReader.
+sbazooka.
+Qed.
+
+Lemma fixedSizeBYTE : fixedSizeReader readBYTE 1.
+Proof.
+  rewrite /fixedSizeReader. move => p q b.
+  destruct p; simpl.
+  + sdestructs => b0 -> H1. sbazooka.
+  + sbazooka.
+Qed.
+
+
+Instance FixedMemIsBYTE : FixedMemIs 1 (readerMemIs BYTE).
+Proof. apply fixedSizeBYTE. Qed.
+
+Lemma memIsBYTE_next_entails (p:ADDR) q (v:BYTE) :
+  p -- q :-> v |-- q = next p /\\ p -- q :-> v.
+Proof. have MI := @memIsFixed _ _ _ FixedMemIsBYTE p q v.
+by simpl (apart _ _ _) in MI.
+Qed.
+
+(*---------------------------------------------------------------------------
+   MemIs for unit type
+  ---------------------------------------------------------------------------*)
+
+Definition unitMemIs (p q: ADDRCursor) (v: unit) := p = q /\\ empSP.
+
+Lemma unitMemIsLe p q v : unitMemIs p q v |-- leCursor p q /\\ unitMemIs p q v.
+Proof. rewrite /unitMemIs. sdestruct => ->. rewrite leCursor_refl. sbazooka. Qed.
+
+Global Instance UnitMemIs : MemIs unit := Build_MemIs unitMemIsLe.
+
+(*---------------------------------------------------------------------------
+   MemIs for pairs
+  ---------------------------------------------------------------------------*)
+
+Section PairMemIs.
+
+  Context {X Y} {MX: MemIs X} {MY: MemIs Y}.
+
+  Definition pairMemIs :=
+    fun p q (v: X*Y) => Exists p', p -- p' :-> (fst v) ** p' -- q :-> (snd v).
+
+  Lemma pairMemIsLe p q v : pairMemIs p q v |-- leCursor p q /\\ pairMemIs p q v.
+  Proof. rewrite /pairMemIs. sdestruct => p'. destruct v as [x y]. rewrite /fst/snd.
+  rewrite -> memIsLe. sdestruct => LE1. rewrite -> (@memIsLe _ _ p'). sdestruct => LE2.
+  rewrite (leCursor_trans LE1 LE2). sbazooka.
+  Qed.
+
+  Global Instance PairMemIs : MemIs (X*Y) := Build_MemIs pairMemIsLe.
+
+  Lemma pairMemIsSimpl p q (v : X*Y) :
+    p -- q :-> v -|- Exists p', p -- p' :-> v.1 ** p' -- q :-> v.2.
+  Proof. by rewrite {1}/memIs/PairMemIs/pairMemIs. Qed.
+
+  Lemma pairMemIsPair p q (x: X) (y: Y) :
+    p -- q :-> (x,y) -|- Exists p', p -- p' :-> x ** p' -- q :-> y.
+  Proof. apply pairMemIsSimpl. Qed.
+
+  Lemma pairMemIsPair' (p q: ADDR) (x: X) (y: Y) :
+    p -- q :-> (x,y) -|- Exists p':ADDR, p -- p' :-> x ** p' -- q :-> y.
+  Proof. rewrite pairMemIsPair. 
+  split; sdestruct => p'. 
+  - destruct p'. sbazooka. rewrite -> memIsFromTop. sbazooka. 
+  - apply lexistsR with p'. sbazooka.
+  Qed.
+
+
+(*
+  Context (dx dy: DWORD) {FX: FixedMemIs dx MX} {FY: FixedMemIs dy MY}.
+  Instance FixedMemIsPair : FixedMemIs (addB dx dy) PairMemIs.
+  Proof. move => p q [x y].
+  rewrite pairMemIsPair. sdestruct => p'.
+  rewrite -> (@memIsFixed _ dx _ _ p).
+  rewrite -> (@memIsFixed _ dy _ _ p').
+  sdestructs => Dx Dy.
+  rewrite -> (@memIsLe _ _ p).
+  rewrite -> (@memIsLe _ _ p').
+  sdestructs => Lx Ly.
+  rewrite (cursorSub_addB Lx Ly Dx Dy). sbazooka.
+  Qed.
+*)
+
+End PairMemIs.
+
+(*---------------------------------------------------------------------------
+   MemIs for sequences
+  ---------------------------------------------------------------------------*)
+
+Section SeqMemIs.
+
+  Context {X} {MX: MemIs X}.
+
+  Definition optionMemIs p q (v: option X) :=
+    match v with
+    | Some v => p -- q :-> v
+    | None => p = q /\\ empSP
+  end.
+
+  Lemma optionMemIsLe p q v : optionMemIs p q v |-- leCursor p q /\\ optionMemIs p q v.
+  Proof. elim v.
+  + move => x. apply memIsLe.
+  + simpl. sdestruct => ->. sbazooka. by rewrite leCursor_refl.
+  Qed.
+
+  Global Instance OptionMemIs : MemIs (option X) := Build_MemIs optionMemIsLe.
+
+  Fixpoint seqMemIs p q (vs: seq X) :=
+    match vs with
+    | v::vs => Exists p', p -- p' :-> v ** seqMemIs p' q vs
+    | nil => p = q /\\ empSP
+    end.
+
+  Lemma seqMemIsLeAux vs : forall p q, seqMemIs p q vs |-- leCursor p q /\\ seqMemIs p q vs.
+  Proof. elim vs.
+  + move => p q. rewrite /seqMemIs. sdestruct => ->. rewrite leCursor_refl. sbazooka.
+  + move => x xs IH p q. rewrite /seqMemIs-/seqMemIs.
+    sdestruct => p'. rewrite -> IH. rewrite -> memIsLe. sdestructs => LE1 LE2.
+    rewrite (leCursor_trans LE1 LE2). sbazooka.
+  Qed.
+
+  Definition seqMemIsLe p q vs := @seqMemIsLeAux vs p q.
+
+  Global Instance SeqMemIs : MemIs (seq X) := Build_MemIs seqMemIsLe.
+
+  Lemma seqMemIsSimpl (p q:ADDRCursor) (xs: seq X):
+    p -- q :-> xs -|- if xs is x::xs then Exists p', p -- p' :-> x ** p' -- q :-> xs
+                                       else p = q /\\ empSP.
+  Proof. case xs.
+  + by rewrite /memIs/SeqMemIs/seqMemIs.
+  + move => x xs'. rewrite /memIs/SeqMemIs/seqMemIs-/seqMemIs. by rewrite /memIs/SeqMemIs.
+  Qed.
+
+  Lemma seqMemIsCons (p q:ADDRCursor) (x:X) (xs: seq X):
+    p -- q :-> (x::xs) -|- Exists p', p -- p' :-> x ** p' -- q :-> xs.
+  Proof. apply seqMemIsSimpl. Qed.
+
+
+  Lemma seqMemIsCons' (p q:ADDR) (x:X) (xs: seq X):
+    p -- q :-> (x::xs) -|- Exists p':ADDR, p -- p' :-> x ** p' -- q :-> xs.
+  Proof. rewrite seqMemIsSimpl. split. sdestruct => p'. destruct p'. sbazooka.
+  rewrite -> memIsFromTop. sbazooka. sbazooka. 
+  Qed. 
+
+  Context {n} {MY: FixedMemIs n MX}.
+
+  Lemma seqFixedMemIsCons' (p q:ADDR) (x:X) (xs: seq X):
+    p -- q :-> (x::xs) -|- p -- (p+#n) :-> x ** (p +#n) -- q :-> xs.
+  Proof. rewrite seqMemIsCons. 
+  split. 
+  - sdestruct => p'. destruct p'. 
+    + rewrite -> memIsFixed. sdestruct => AP. rewrite (apart_addBn AP). sbazooka.
+    + rewrite -> memIsFromTop. sbazooka. 
+  - sbazooka.
+  Qed. 
+
+  Lemma seqMemIsNil (p q:ADDRCursor):
+    p -- q :-> (nil:seq X) -|- p = q /\\ empSP.
+  Proof. apply seqMemIsSimpl. Qed.
+
+  Lemma seqMemIsCat p q (xs ys : seq X):
+    p -- q :-> (xs ++ ys) -|- p -- q :-> (xs, ys).
+  Proof.
+    elim: xs p => [|x xs IHxs] p.
+    - rewrite pairMemIsSimpl/fst/snd cat0s. split. sbazooka. erewrite seqMemIsNil. sbazooka.
+      sdestructs => p'. rewrite seqMemIsNil. sdestructs => ->. sbazooka.
+    - simpl ((x::xs) ++ ys). split.
+      + rewrite pairMemIsSimpl seqMemIsCons /fst/snd.
+        setoid_rewrite IHxs. sdestruct => p'. rewrite pairMemIsSimpl /fst/snd.
+        sdestruct => q'.
+        apply lexistsR with q'. rewrite seqMemIsCons. ssimpl.
+        apply lexistsR with p'. sbazooka.
+      + rewrite pairMemIsSimpl /fst/snd. sdestruct => p'.
+        rewrite seqMemIsCons. rewrite seqMemIsCons.
+        setoid_rewrite IHxs. sdestruct => q'. apply lexistsR with q'.
+        rewrite pairMemIsSimpl. rewrite /fst/snd. ssimpl.
+        apply lexistsR with p'. sbazooka.
+  Qed.
+
+End SeqMemIs.
+
+
+Lemma seqFixedMemIsConsNE X `(FMI:FixedMemIs X) (p q : ADDR) (v:X) vs : 0 < n < 2^naddrBits -> 
+    p -- q :-> (v::vs) |-- p != q /\\ memIs p q (v::vs).
+Proof. move/andP => [GT LT]. case E: n => [|n']; subst => //. 
+  rewrite -> seqFixedMemIsCons'. 
+  have H: p != p+#n'.+1. by apply: addBn_ne. 
+  (* Why can't I identify the right memIs? *)
+  rewrite -> memIsLe at 1. sdestruct => H1. 
+  rewrite sepSPC. 
+  rewrite -> memIsLe at 1. sdestruct => H2. 
+  rewrite leCursor_nat in H1.
+  rewrite leCursor_nat in H2.
+  rewrite leq_eqVlt in H1. 
+  have HI:= @cursorToNat_inj _ p (p+#n'.+1). 
+  case E: (cursorToNat p == cursorToNat (p+#n'.+1)). 
+  rewrite (eqP E) in HI. specialize (HI (refl_equal _)). injection HI => HI'. rewrite {1}HI' in H. 
+  by rewrite eq_refl in H. rewrite E orFb in H1. 
+  have NE: cursorToNat p != cursorToNat q. apply negbT. apply: ltn_eqF. by apply: leq_trans H2. 
+  rewrite inj_eq in NE; last by apply cursorToNat_inj.
+  rewrite NE.
+  sbazooka.  
+Qed. 
+
+(*---------------------------------------------------------------------------
+   MemIs for subtype
+  ---------------------------------------------------------------------------*)
+
+Section SubMemIs.
+
+  Context {X} {MX : MemIs X}.
+
+  Definition subMemIs P p q (v: {x:X | P x}) := p -- q :-> sval v.
+  Implicit Arguments subMemIs [].
+
+  Lemma subMemIsLe P p q v : subMemIs P p q v |-- leCursor p q /\\ subMemIs P p q v.
+  Proof. rewrite /subMemIs. apply memIsLe. Qed.
+
+  Global Instance SubMemIs P : MemIs {x : X | P x} := Build_MemIs (@subMemIsLe P).
+
+  Lemma subMemIsSub P p q (v: {x:X | P x}) : p -- q :-> v |-- p -- q :-> sval v.
+  Proof. by rewrite /=/subMemIs. Qed.
+
+  Lemma seqSubMemIsMapAux P (vs: seq {x:X | P x}) : forall p q,
+     p -- q :-> vs -|- p -- q :-> map sval vs.
+  Proof. elim vs.
+  + move => p q. rewrite !seqMemIsNil. sbazooka.
+  + move => v vs' IH p q.
+    rewrite !seqMemIsCons. split.
+    - sdestruct => q'. apply lexistsR with q'. rewrite <- subMemIsSub.
+      by rewrite -IH.
+    - sdestruct => p'. rewrite -IH. apply lexistsR with p'. ssimpl. reflexivity.
+  Qed.
+
+  Lemma seqSubMemIs P p q (vs: seq {x:X | P x}) : p -- q :-> vs -|- p -- q :-> map sval vs.
+  Proof. apply seqSubMemIsMapAux. Qed.
+
+End SubMemIs.
+
+Lemma seq_BYTE_size (p q: ADDR) (vs: seq BYTE) :
+  p -- q :-> vs |-- q = p +# size vs /\\ p -- q :-> vs.
+Proof.
+  elim: vs p => [|b bs IHbs] p.
+  - rewrite -> seqMemIsNil. sdestruct => [[<-]]. ssplits => //.
+    by rewrite addB0.
+  - rewrite -> seqMemIsCons. rewrite /size -/size. sdestruct => [[p'|]].
+    - rewrite ->IHbs. sdestruct => Hq. rewrite ->memIsBYTE_next_entails.
+      sdestruct => Hp'. symmetry in Hp'. subst. ssplit; last by sbazooka.
+      clear IHbs. replace (p +# (size bs).+1) with (incB p +# size bs).
+      apply nextIsInc in Hp'. subst. rewrite <-addB_addn. rewrite -addB1.
+      by rewrite ->addB_addn. rewrite -addB1. rewrite <-addB_addn. by rewrite add1n.
+    - rewrite -> memIsFromTop.  rewrite lfalse_is_exists. sdestruct => [[]].
+Qed.
+
+Lemma seqMemIsBYTE_addn (vs:seq BYTE) : forall m (p:ADDR),
+  m < 2^naddrBits ->
+  p -- (p+#m) :-> vs |--
+  size vs = m /\\ p -- (p+#m) :-> vs.
+Proof.
+  induction vs => m p BOUND.
+(* vs is nil *)
+  setoid_rewrite seqMemIsNil.
+  sdestruct => EQ.
+  have H: m = 0.
+  apply (addB0_inv (p:=p) BOUND). have: p = p +# m by congruence. by move => {1}->.
+  rewrite H addB0. sbazooka.
+(* vs is non-nil *)
+  setoid_rewrite seqMemIsCons.
+  sdestruct => p'.
+  rewrite -> memIsBYTE_next_entails.
+  sdestruct => ->.
+
+  destruct m as [|m].
+    rewrite addB0. rewrite -> (@memIsLe _ _ (next p)). rewrite leCursor_next /ltCursor.
+    rewrite ltB_nat ltnn.  rewrite lpropandF. by ssimpl.
+    simpl (size _). apply ltnW in BOUND.
+    specialize (IHvs m (p+#1) BOUND). rewrite <- addB_addn in IHvs. rewrite add1n in IHvs.
+
+    case E: (next p) => [q |].
+      symmetry in E. have NI := nextIsInc (sym_equal E). subst.
+      rewrite -> IHvs. sbazooka.  congruence.
+      rewrite -> memIsFromTop. by ssimpl.
+Qed.
+
+
+Lemma fixedSizeReader_bind T1 T2 (r1: Reader T1) (r2: T1 -> Reader T2) n1 n2 :
+  fixedSizeReader r1 n1 ->
+  (forall x, fixedSizeReader (r2 x) n2) ->
+  fixedSizeReader (readerBind r1 r2) (n1+n2).
+Proof. move => F1 F2.
+move => p q v.
+rewrite /fixedSizeReader in F1, F2. rewrite interpReader_bind.
+sdestructs => p' v1. rewrite -> F1.
+sdestruct => E1.
+rewrite -> F2.
+sdestruct => E2.
+have A := (apart_addn E1 E2). sbazooka.
+Qed.
+
+Lemma fixedSizeReader_bind_retn T1 T2 (r1: Reader T1) n1 (f: T1 -> T2) :
+  fixedSizeReader r1 n1 ->
+  fixedSizeReader (readerBind r1 (fun x => readerRetn (f x))) n1.
+Proof. move => F1.
+move => p q v.
+rewrite /fixedSizeReader in F1. rewrite interpReader_bind.
+sdestructs => p' v1. rewrite -> F1.
+sdestruct => E1.
+rewrite interpReader_retn.
+sbazooka. subst. done. erewrite interpReader_retn. sbazooka.
+Qed.
+
+Lemma fixedSizeReader_retn T (x:T) : fixedSizeReader (readerRetn x) 0.
+Proof. rewrite /fixedSizeReader. move => p q v. simpl. sbazooka. Qed.
+
+Lemma fixedSizeDWORD : fixedSizeReader readDWORD 4.
+Proof.
+  rewrite /fixedSizeReader. move => p q b.
+  do 4 apply (fixedSizeReader_bind fixedSizeBYTE) => ?.
+  apply fixedSizeReader_retn.
+Qed.
+
+Instance FixedMemIsDWORD : FixedMemIs 4 (readerMemIs DWORD).
+Proof. apply fixedSizeDWORD. Qed.
+
+Lemma fixedSizeQWORD : fixedSizeReader readQWORD 8.
+Proof.
+  rewrite /fixedSizeReader. move => p q b.
+  do 8 apply (fixedSizeReader_bind fixedSizeBYTE) => ?.
+  apply fixedSizeReader_retn.
+Qed.
+
+Instance FixedMemIsQWORD : FixedMemIs 8 (readerMemIs QWORD).
+Proof. apply fixedSizeQWORD. Qed.
+
+
+Lemma fixedSizeWORD : fixedSizeReader readWORD 2.
+Proof.
+  rewrite /fixedSizeReader. move => p q b.
+  rewrite /readWORD.
+  apply (fixedSizeReader_bind fixedSizeBYTE) => b0.
+  apply (fixedSizeReader_bind fixedSizeBYTE) => b1.
+  apply fixedSizeReader_retn.
+Qed.
+
+Instance FixedMemIsWORD : FixedMemIs 2 (readerMemIs WORD).
+Proof. apply fixedSizeWORD. Qed.
+
+Lemma fixedSizeTupleBYTE n : fixedSizeReader (readTupleBYTE n) n.
+Proof.
+induction n => //=.
++ by apply fixedSizeReader_retn.
++ apply (fixedSizeReader_bind fixedSizeBYTE) => b0.
+  by apply fixedSizeReader_bind_retn.
+Qed.
+
+Instance FixedMemIsTupleBYTE n : FixedMemIs n (readerMemIs (n.-tuple BYTE)).
+Proof. apply fixedSizeTupleBYTE. Qed.
+
+
+Corollary memIsDWORD_range (p q: ADDR) (c:DWORD):
+  p -- q :-> c -|- q = p +# 4 /\\ p -- q :-> c.
+Proof. split; last by sdestruct.
+have FMI := FixedMemIsDWORD.  rewrite /FixedMemIs in FMI. specialize (FMI p q c).
+etransitivity; first apply FMI. (* Why doesn't rewrite work here? *)
+sdestruct => A.
+sbazooka. by apply apart_addBn.
+Qed.
+
+(*---------------------------------------------------------------------------
+   Logical interpretation of writers
+  ---------------------------------------------------------------------------*)
+
+Fixpoint interpWriterTm {T} (wt:WriterTm T) (p q: ADDRCursor) (t: T) :=
+  match wt with
+  | writerRetn t' => t = t' /\\ p = q /\\ empSP
+  | writerNext b wt' =>
+      (* We can't write beyond the last byte of memory! *)
+      if p is mkCursor p'
+      then byteIs p' b ** interpWriterTm wt' (next p') q t
+      else lfalse
+  | writerSkip wt' =>
+      if p is mkCursor p'
+      then Exists b, byteIs p' b ** interpWriterTm wt' (next p') q t
+      else lfalse
+  | writerCursor wt' => interpWriterTm (wt' p) p q t
+  | writerFail => lfalse
+  end.
+
+Lemma interpWriterTm_roundtrip X T (wt: WriterTm T) (R: Reader X) p q x t:
+  simrw x p R wt ->
+  interpWriterTm wt p q t |-- p -- q :-> x.
+Proof.
+  intros Hsim. induction Hsim => //; rewrite /interpWriterTm-/interpWriterTm/=.
+  - sbazooka.
+  - apply lexistsR with b. ssimpl. apply IHHsim.
+  - sdestructs => b. apply lexistsR with b. ssimpl. apply IHHsim.
+  - done.
+  - done.
+  - done.
+Qed.
+
+Lemma memIsBYTE_byteIs (p:ADDR) q b : p -- q :-> b |-- byteIs p b.
+Proof.
+rewrite readerMemIsSimpl interpReader_bindBYTE.
+rewrite /interpReader. sdestructs => b' -> _. by ssimpl.
+Qed.
+
+
+Lemma runWriterTm_memIs T (W: WriterTm T) p q t bytes:
+  runWriterTm true W p = Some (t, bytes) ->
+  p -- q :-> bytes |-- interpWriterTm W p q t.
+Proof.
+  revert p bytes. induction W => p bytes //.
+  - case => <- <- /=. sdestruct => ->. sbazooka.
+  - destruct p as [p|]; last done.
+    remember (runWriterTm true W (next p)) as runw.
+    destruct runw as [[q' bytes']|] => // Hinj.
+    rewrite /= in Hinj. rewrite -Heqrunw in Hinj. rewrite /interpWriterTm-/interpWriterTm.
+    injection Hinj => ? ? {Hinj}. subst bytes q'.
+    rewrite <- (IHW _ bytes'); last by rewrite Heqrunw. 
+  rewrite -> seqMemIsCons. sdestruct => q'. 
+  rewrite -> memIsBYTE_next_entails. sdestruct => ->. rewrite -> memIsBYTE_byteIs. by ssimpl.
+    simpl in Hinj. by rewrite -Heqrunw in Hinj.
+  - destruct p => //= H.
+    case E: (runWriterTm true W (next p)) => [[x bytes'] |].
+    * rewrite E in H. injection H => [H1 H2]. subst. specialize (IHW _ _ E).
+      simpl. apply lexistsR with #0. sdestructs => q1 b' H1 H2. subst.
+      sbazooka.
+    * by rewrite E in H.
+  - move => /=SF. apply: H => //.
+Qed.
+
+Lemma interpWriterTm_bind {X Y} (w1: WriterTm X) (w2: X -> WriterTm Y) p q y:
+  interpWriterTm (let! x = w1; w2 x) p q y -|-
+  Exists p', Exists x, interpWriterTm w1 p p' x ** interpWriterTm (w2 x) p' q y.
+Proof.
+  revert p. induction w1 => p //=.
+  - sbazooka. subst. sbazooka.
+  - destruct p.
+    * split.
+      - rewrite IHw1. by sbazooka.
+      - sdestructs => p' v. rewrite IHw1. by sbazooka.
+    * split; first done. by sbazooka.
+  - destruct p.
+    * split.
+      - sdestruct => b. rewrite IHw1. by sbazooka.
+      - sdestructs => p' v b. apply lexistsR with b. rewrite IHw1. by sbazooka.
+    * split; first done. by sbazooka.
+  - split; first done. by sbazooka.
+Qed.
+
+Lemma interpWriterTm_retn {X} (p q: ADDRCursor) (t t':X) :
+  interpWriterTm (writerRetn t) p q t' -|- (t' = t /\\ p = q /\\ empSP).
+Proof.  simpl. reflexivity. Qed.
+
+Lemma interpWriterTm_getWCursor (p q r: ADDRCursor) :
+  interpWriterTm getWCursor p q r -|- p = q /\\ q = r /\\ empSP.
+Proof. simpl. split; sdestructs => H1 H2; subst; sbazooka. Qed.
+
+Lemma interpWriterTm_writerFail (p q: ADDRCursor) :
+  interpWriterTm writerFail p q tt -|- lfalse.
+Proof. reflexivity. Qed.
+
+
+Lemma interpWriterTm_top T (wt: WriterTm T) t (q: ADDR) :
+  interpWriterTm wt (top _) q t -|-
+  lfalse.
+Proof.
+  split; last done. induction wt => //=.
+  sdestructs. discriminate.
+Qed.
+
+(* This could also be an instance of memIs just like readerMemIs, but we don't
+   want typeclass resolution to be ambiguous. *)
+Definition interpWriter X {W: Writer X} (p q: ADDRCursor) (x: X) :=
+  interpWriterTm (W x) p q tt.
+
+Lemma interpWriter_roundtrip X (W: Writer X) (R: Reader X)
+      {RT: Roundtrip R W} p q x:
+  interpWriter p q x |-- p -- q :-> x.
+Proof.
+  exact: interpWriterTm_roundtrip.
+Qed.
+
+Lemma runWriter_interpWriter X (W: Writer X) p q bytes x:
+  runWriter true writeNext p x = Some bytes ->
+  p -- q :-> bytes |-- interpWriter p q x.
+Proof.
+  rewrite /interpWriter /runWriter /writeNext => H. simpl in H.
+  apply: runWriterTm_memIs.
+  destruct (runWriterTm _ (W x) p) as [[[] bytes']|] => //. by congruence.
+Qed.
+
